Phi_Algebras/Phi_Spec_Pre.thy
@@ -13,11 +13,22 @@ lemma Subjection_Id_on:
   \<open>Id_on (S \<s>\<u>\<b>\<j> P) = (Id_on S \<s>\<u>\<b>\<j> P)\<close>
   by (auto simp add: Subjection_expn)
 
+lemma Subjection_image:
+  \<open>f ` (S \<s>\<u>\<b>\<j> P) = (f ` S \<s>\<u>\<b>\<j> P)\<close>
+  by (auto simp add: Subjection_expn)
+
 definition ExSet :: " ('c \<Rightarrow> 'a set) \<Rightarrow> 'a set" (binder "\<exists>*" 14)
   where "ExSet S = {p. (\<exists>c. p \<in> S c)}"
 notation ExSet (binder "\<exists>\<^sup>s" 14)
 
 lemma ExSet_expn: "p \<in> ExSet S \<longleftrightarrow> (\<exists>c. p \<in> S c)" unfolding ExSet_def by simp
 
+lemma ExSet_Id_on:
+  \<open>Id_on (ExSet S) = ExSet (\<lambda>x. Id_on (S x))\<close>
+  by (auto simp add: ExSet_expn; blast)
+
+lemma ExSet_image:
+  \<open>f ` (ExSet S) = (ExSet (\<lambda>c. f ` S c))\<close>
+  by (auto simp add: ExSet_expn image_iff Bex_def; blast)
 
 end
