Phi_Semantics/PhiSem_Mem_C_Base.thy
@@ -55,8 +55,10 @@ lemma index_offset_bound_strict:
 section \<open>Fiction\<close>
 
 debt_axiomatization Map_of_Val :: \<open>VAL \<Rightarrow> nat list \<rightharpoonup> VAL\<close>
+                and Dom_of_TY :: \<open>TY \<Rightarrow> nat list set\<close>
   where Map_of_Val_inj: \<open>Va \<in> Well_Type T \<Longrightarrow> Vb \<in> Well_Type T \<Longrightarrow> Map_of_Val Va = Map_of_Val Vb \<Longrightarrow> Va = Vb\<close>
-  and   Map_of_Val_same_dom: \<open>Va \<in> Well_Type T \<Longrightarrow> Vb \<in> Well_Type T \<Longrightarrow> dom (Map_of_Val Va) = dom (Map_of_Val Vb)\<close>
+  and   Map_of_Val_dom: \<open>Va \<in> Well_Type T \<Longrightarrow> dom (Map_of_Val Va) = Dom_of_TY T\<close>
+  and   Dom_of_TY_step: \<open>valid_idx_step T i \<Longrightarrow> Well_Type T \<noteq> {} \<Longrightarrow> Dom_of_TY (idx_step_type i T) \<subseteq> Dom_of_TY T\<close>
   and   Mapof_not_1[simp]: \<open>Map_of_Val V \<noteq> 1\<close>
   and   Map_of_Val_pull_step: \<open>valid_idx_step T i \<Longrightarrow> V \<in> Well_Type T
                           \<Longrightarrow> pull_map [i] (Map_of_Val V) = Map_of_Val (idx_step_value i V)\<close>
@@ -66,6 +68,10 @@ debt_axiomatization Map_of_Val :: \<open>VAL \<Rightarrow> nat list \<rightharpo
 lemma Map_of_Val_pull:
   \<open>valid_index T idx \<Longrightarrow> V \<in> Well_Type T \<Longrightarrow> pull_map idx (Map_of_Val V) = Map_of_Val (index_value idx V)\<close>
   by (induct idx arbitrary: V T; simp; metis Map_of_Val_pull_step idx_step_value_welltyp pull_map_cons)
+
+lemma Dom_of_TY:
+  \<open>valid_index T idx \<Longrightarrow> Well_Type T \<noteq> {} \<Longrightarrow> Dom_of_TY (index_type idx T) \<subseteq> Dom_of_TY T\<close>
+  by (induct idx arbitrary: T; simp; meson Dom_of_TY_step dual_order.trans valid_idx_valid_typ_step)
 
 lemma total_Mapof_disjoint:
    \<open>g ## (push_map idx (to_share \<circ> h))
@@ -84,12 +90,12 @@ lemma Map_of_Val_mod:
 \<Longrightarrow> u \<in> Well_Type (index_type idx T)
 \<Longrightarrow> Map_of_Val (index_mod_value idx (\<lambda>_. u) v) = Map_of_Val v ++ push_map idx (Map_of_Val u)\<close>
   apply (induct idx arbitrary: u v T; simp)
-  using Map_of_Val_same_dom map_add_subsumed_dom apply (metis order_refl)
+  using Map_of_Val_dom map_add_subsumed_dom apply (metis order_refl)
   by clarify (simp add: idx_step_value_welltyp Map_of_Val_mod_step  push_map_distrib_map_add
                         Map_of_Val_pull_step[symmetric] push_pull_map map_add_subsumed2
                         push_map_push_map)
 
-lemma Map_of_Val_modify_fiction:
+(* lemma Map_of_Val_modify_fiction:
    \<open>valid_index T idx
 \<Longrightarrow> v \<in> Well_Type T
 \<Longrightarrow> u \<in> Well_Type (index_type idx T)
@@ -114,7 +120,7 @@ lemma Map_of_Val_modify_fiction:
 (* lemma pull_map_share_Mapof_not_eq_1[simp]:
   \<open>valid_index (Typeof v) idx \<Longrightarrow> pull_map idx (share n (to_share \<circ> Map_of_Val v)) = 1 \<longleftrightarrow> n = 0\<close>
   by (cases \<open>n = 0\<close>; simp add: pull_map_share pull_map_to_share Map_of_Val_pull)
-*)
+*)*)
 
 
 lemma map_add_restrict_itself [simp]: \<open>(f ++ g) |` dom g = g\<close>
@@ -128,7 +134,7 @@ proof (rule Map_of_Val_inj, assumption)
      and tyB: \<open>Vb \<in> Well_Type T\<close>
      and feq: \<open>f ++ Map_of_Val Va = f ++ Map_of_Val Vb\<close>
   then have \<open>(f ++ Map_of_Val Va) |` dom (Map_of_Val Va) = (f ++ Map_of_Val Vb) |` dom (Map_of_Val Vb)\<close>
-    using Map_of_Val_same_dom by metis 
+    using Map_of_Val_dom by metis 
   note this [simplified]
   then show \<open>Map_of_Val Va = Map_of_Val Vb\<close> .
 qed
@@ -140,7 +146,7 @@ lemma Val_of_Map_append[simp]:
   unfolding Val_of_Map_def
   using someI[where P=\<open>\<lambda>V. (\<exists>fa. fa ++ Map_of_Val V = f ++ Map_of_Val v) \<and> V \<in> Well_Type T\<close> and x=v, simplified]
         Map_of_Val_inj_plus
-  by (metis (no_types, lifting) Map_of_Val_same_dom map_add_restrict_itself) 
+  by (metis (no_types, lifting) Map_of_Val_dom map_add_restrict_itself) 
 
 lemmas Val_of_Map[simp] = Val_of_Map_append[where f = \<open>Map.empty\<close>, simplified]
 
@@ -151,32 +157,481 @@ definition Map_of_Val_ins
 definition Map_of_Val_ins_dom
   where \<open>Map_of_Val_ins_dom TY = {x. pred_option (\<lambda>x'. nosep.dest x' \<in> Well_Type TY) x}\<close>
 
+lemma Map_of_Val_ins_eval[simp]:
+  \<open>Map_of_Val_ins (Some (nosep u)) = (map_option nosep) o Map_of_Val u\<close>
+  unfolding Map_of_Val_ins_def by simp
+
+lemma Map_of_Val_ins_dom_eval[simp]:
+  \<open>Some (nosep u) \<in> Map_of_Val_ins_dom TY \<longleftrightarrow> u \<in> Well_Type TY\<close>
+  unfolding Map_of_Val_ins_dom_def by simp
+
 
 interpretation Map_of_Val_ins: cancl_sep_insertion_monoid \<open>Map_of_Val_ins\<close> \<open>Map_of_Val_ins_dom TY\<close>
-  apply (standard; auto simp add: Map_of_Val_ins_def fun_eq_iff split_option_ex times_fun
-                                  sep_disj_fun_def split_nosep_meta_all Map_of_Val_ins_dom_def
-                        split: option.split)
+  apply (standard; clarsimp simp add: Map_of_Val_ins_def split_nosep_meta_all
+                                      Map_of_Val_ins_dom_def
+                            split: option.split)
+
+  apply (auto simp add: fun_eq_iff split_option_ex times_fun 
+                                  sep_disj_fun_def split_nosep_meta_all
+                        split: option.split)[1]
   using Mapof_not_1 apply fastforce
-  apply (metis Map_of_Val_same_dom domIff one_option_def option.exhaust_sel option.map_disc_iff sep_disj_option_nonsepable(1) sep_no_inverse)
+  apply (metis Map_of_Val_dom domIff option.map_disc_iff times_option(2))
   subgoal premises prems for a x x' proof -
     have t1: \<open>a x = 1\<close> for x
-      by (metis Map_of_Val_same_dom domIff one_option_def option.exhaust_sel option.map_disc_iff prems(1) prems(2) prems(3) prems(4) sep_disj_option_nonsepable(1) sep_no_inverse)
+      by (metis Map_of_Val_dom domIff one_option_def option.map_disc_iff prems(1) prems(2) prems(3) prems(4) times_option(2))
     have t2: \<open>map_option nosep o Map_of_Val x = map_option nosep o Map_of_Val x'\<close>
       using prems(4) t1 by auto
     show ?thesis
       by (metis (mono_tags, lifting) Map_of_Val_inj fun.inj_map_strong nosep.inject option.inj_map_strong prems(2) prems(3) t2) 
   qed .
 
-interpretation Map_of_Val_shared_ins: cancl_perm_ins_homo \<open>((o) to_share) o Map_of_Val_ins\<close> \<open>Map_of_Val_ins_dom TY\<close>
-  by (standard; simp add: pointwise_set_UNIV)
-
-thm Map_of_Val_ins.\<F>_functional_refinement
-thm Map_of_Val_shared_ins.\<F>_functional_refinement
 
 
-interpretation Map_of_Val': kernel_is_1 \<open>Map_of_Val' TY\<close>
-  by (standard, clarsimp simp add: split_option_all Map_of_Val'_def split_nosep_meta_all fun_eq_iff,
-      insert Mapof_not_1, fastforce)
+lemma map_tree_refinement_modify:
+  \<open> dom a = dom b \<and> dom b \<subseteq> D
+\<Longrightarrow> (\<And>r. r ## push_map idx a \<and> r ## push_map idx b \<and> r * push_map idx a \<in> S \<Longrightarrow> r * push_map idx b \<in> S)
+\<Longrightarrow> Id_on UNIV * ({(a, a ++ push_map idx b)} \<s>\<u>\<b>\<j> a. dom a = D)
+    \<r>\<e>\<f>\<i>\<n>\<e>\<s> { (push_map idx a, push_map idx b)}
+    \<w>.\<r>.\<t> \<F>_functional id S
+    \<i>\<n> { push_map idx a }\<close>
+  for a :: \<open>'a list \<Rightarrow> VAL nosep option\<close>
+  unfolding Fictional_Forward_Simulation_def the_subtree_def
+  apply (clarsimp simp add: Subjection_expn set_mult_expn ExSet_expn)
+  subgoal premises prems for r R a' u x
+  proof -
+    have t1: \<open>dom x \<inter> dom (idx \<^enum>\<^sub>m b) = {}\<close>
+      using disjoint_iff prems(10) sep_disj_partial_map_disjoint by fastforce
+    have t2: \<open>dom r \<inter> dom (idx \<^enum>\<^sub>m b) = {}\<close>
+      by (metis prems(2) prems(4) push_map_dom_eq sep_disj_partial_map_disjoint)
+    have t3: \<open>dom u \<inter> dom (idx \<^enum>\<^sub>m b) = {}\<close>
+      by (metis prems(12) prems(2) push_map_dom_eq sep_disj_partial_map_disjoint)
+    have t4: \<open>u ## idx \<^enum>\<^sub>m b\<close>
+      using sep_disj_partial_map_disjoint t3 by blast
+    have t5: \<open>r ## idx \<^enum>\<^sub>m b\<close>
+      using sep_disj_partial_map_disjoint t2 by blast
+    have t6: \<open>dom x \<inter> dom a' = {}\<close>
+      by (meson prems(9) sep_disj_partial_map_disjoint)
+    show ?thesis
+      apply (simp add: t5, rule exI[where x=u], simp add: t4 prems)
+      by (smt (verit, best) map_add_subsumed_dom mult.left_commute prems(1) prems(2) prems(4) prems(6) prems(8) push_map_distrib_map_add t1 t2 t3 t5 times_fun_map_add_right verit_comp_simplify1(2))
+  qed .
+
+
+
+thm Map_of_Val_ins.\<F>_functional_refinement_complex[simplified]
+thm refinement_frame[OF Map_of_Val_ins.\<F>_functional_refinement_complex[simplified]]
+thm sep_refinement_stepwise[
+      OF refinement_frame[OF Map_of_Val_ins.\<F>_functional_refinement_complex[simplified]],
+      where Ib = \<open>\<F>_it\<close>, simplified]
+
+thm Map_of_Val_ins.\<F>_functional_projection
+
+
+lemma \<F>_it_refinement_projection_'UNIV:
+        \<open> UNIV * S \<subseteq> S'
+      \<Longrightarrow> refinement_projection \<F>_it S \<subseteq> UNIV * S'\<close>
+        for S :: \<open>'a::sep_monoid set\<close> and S'
+        using \<F>_it_refinement_projection[where S=\<open>UNIV * S\<close>, unfolded refinement_projection_UNIV_times_D] .
+
+lemma fiction_Map_of_Val_ins_comp_id_simp:
+  \<open>(\<F>_functional Map_of_Val_ins (Map_of_Val_ins_dom TY) \<Zcomp>\<^sub>\<I>
+    \<F>_functional id (Map_of_Val_ins ` Map_of_Val_ins_dom TY))
+  = \<F>_functional Map_of_Val_ins (Map_of_Val_ins_dom TY)\<close>
+  by (rule \<F>_functional_comp[where f=id, simplified, symmetric]; clarsimp)
+
+lemma val_map_eq_index_value_eq:
+  \<open>valid_index TY idx \<Longrightarrow>
+    u_idx \<in> Well_Type (index_type idx TY) \<Longrightarrow>
+    v \<in> Well_Type TY \<Longrightarrow>
+    map_option nosep \<circ> Map_of_Val v = u * idx \<^enum>\<^sub>m (map_option nosep \<circ> Map_of_Val u_idx) \<Longrightarrow>
+    u ## idx \<^enum>\<^sub>m (map_option nosep \<circ> Map_of_Val u_idx) \<Longrightarrow>
+    index_value idx v = u_idx \<close>
+  subgoal premises prems proof -
+    have t1: \<open>dom (pull_map idx (Map_of_Val v)) = Dom_of_TY (index_type idx TY)\<close>
+      using Map_of_Val_dom Map_of_Val_pull index_value_welltyp prems(1) prems(3) by auto
+    have t2: \<open>dom (pull_map idx (Map_of_Val v)) =
+              dom (pull_map idx u) \<union> dom (Map_of_Val u_idx)\<close>
+      by (metis dom1_dom dom1_mult dom_map_option_comp map_option_homo_one prems(4) prems(5) pull_map_funcomp pull_map_homo_mult pull_map_sep_disj pull_push_map)
+    have t3: \<open>dom (pull_map idx u) \<inter> dom (Map_of_Val u_idx) = {}\<close>
+      by (metis dom1_dom dom_map_option_comp prems(5) pull_map_sep_disj pull_push_map sep_disj_dom1_disj_disjoint)
+    have t4: \<open>dom (Map_of_Val u_idx) = Dom_of_TY (index_type idx TY)\<close>
+      using Map_of_Val_dom prems(2) by force
+    have t5: \<open>pull_map idx u = 1\<close>
+      using t1 t2 t3 t4 by fastforce
+    then have \<open>pull_map idx (map_option nosep \<circ> Map_of_Val v) = (map_option nosep \<circ> Map_of_Val u_idx)\<close>
+      by (simp add: prems(4) pull_map_homo_mult)
+    then have \<open>pull_map idx (Map_of_Val v) = Map_of_Val u_idx\<close>
+      by (smt (verit) fun.inj_map_strong map_option_homo_one nosep.inject option.inj_map_strong pull_map_funcomp)
+    then show ?thesis
+      by (metis Map_of_Val_inj Map_of_Val_pull index_value_welltyp prems(1) prems(2) prems(3))
+  qed .
+
+lemma val_map_mod_index_value:
+  \<open> valid_index TY idx \<Longrightarrow>
+    x \<in> Well_Type TY \<Longrightarrow>
+    u \<in> Well_Type (index_type idx TY) \<Longrightarrow>
+    v \<in> Well_Type (index_type idx TY) \<Longrightarrow>
+    r ## idx \<^enum>\<^sub>m (map_option nosep \<circ> Map_of_Val u) \<Longrightarrow>
+    r ## idx \<^enum>\<^sub>m (map_option nosep \<circ> Map_of_Val v) \<Longrightarrow>
+    r * idx \<^enum>\<^sub>m (map_option nosep \<circ> Map_of_Val u) = map_option nosep \<circ> Map_of_Val x \<Longrightarrow>
+    r * idx \<^enum>\<^sub>m (map_option nosep \<circ> Map_of_Val v) = map_option nosep \<circ> Map_of_Val (index_mod_value idx (\<lambda>_. v) x)\<close>
+  by (simp add: Map_of_Val_mod map_option_funcomp_map_add,
+      smt (verit) Map_of_Val_dom dom_map_option_comp map_add_subsumed_dom map_le_implies_dom_le map_option_homo_one pull_push_map push_map_dom_eq push_map_homo push_pull_map sep_disj_partial_map_disjoint times_fun_map_add_right)
+
+lemma val_map_mod_index_value_projection:
+  \<open> valid_index TY idx \<Longrightarrow>
+    u_idx \<in> Well_Type (index_type idx TY) \<Longrightarrow>
+    refinement_projection (\<F>_functional id (Map_of_Val_ins ` Map_of_Val_ins_dom TY)) {idx \<^enum>\<^sub>m (map_option nosep \<circ> Map_of_Val u_idx)}
+    \<subseteq> UNIV * Map_of_Val_ins ` Some ` nosep ` {a. index_value idx a = u_idx \<and> a \<in> Well_Type TY}\<close>
+  apply (clarsimp simp add: image_iff set_mult_expn refinement_projection_def
+                            Map_of_Val_ins_dom_def Map_of_Val_ins_def;
+         case_tac xb; simp add: split_nosep_meta_all)
+  apply (smt (verit, best) Mapof_not_1 dom_1 dom_eq_empty_conv dom_map_option_comp)
+  by (metis mult.commute mult_1_class.mult_1_right sep_magma_1_right val_map_eq_index_value_eq)
+
+lemma fiction_Map_of_Val_ins_projection:
+  \<open> valid_index TY idx
+\<Longrightarrow> u_idx \<in> Well_Type (index_type idx TY)
+\<Longrightarrow> refinement_projection (\<F>_functional Map_of_Val_ins (Map_of_Val_ins_dom TY))
+                          {idx \<^enum>\<^sub>m (map_option nosep \<circ> Map_of_Val u_idx)}
+      \<subseteq> UNIV * Some ` nosep ` {a. index_value idx a = u_idx \<and> a \<in> Well_Type TY }\<close>
+  apply (subst fiction_Map_of_Val_ins_comp_id_simp[symmetric])
+  apply (rule refinement_projections_stepwise_UNIV_paired)
+  apply (rule Map_of_Val_ins.\<F>_functional_projection)
+  apply (clarsimp)
+  by (insert val_map_mod_index_value_projection)
+
+lemma fiction_Map_of_Val_ins_projection':
+  \<open> valid_index TY idx
+\<Longrightarrow> u_idx \<in> Well_Type (index_type idx TY)
+\<Longrightarrow> refinement_projection (\<F>_functional Map_of_Val_ins (Map_of_Val_ins_dom TY))
+                          {idx \<^enum>\<^sub>m (map_option nosep \<circ> Map_of_Val u_idx)}
+      \<subseteq> UNIV * Some ` nosep ` {a. index_value idx a = u_idx }\<close>
+  subgoal premises prems proof -
+    have \<open> UNIV * Some ` nosep ` {a. index_value idx a = u_idx \<and> a \<in> Well_Type TY }
+        \<subseteq> UNIV * Some ` nosep ` {a. index_value idx a = u_idx }\<close>
+      by (simp add: Collect_mono_iff image_mono)
+    then show ?thesis
+      using fiction_Map_of_Val_ins_projection prems(1) prems(2) by blast
+  qed .
+
+lemma fiction_Map_of_Val_ins_refinement:
+  \<open> valid_index TY idx
+\<Longrightarrow> Well_Type TY \<noteq> {}
+\<Longrightarrow> v \<in> Well_Type (index_type idx TY)
+\<Longrightarrow> u_idx \<in> Well_Type (index_type idx TY)
+\<Longrightarrow> Id_on UNIV * ({(Some u, (Some o map_nosep (index_mod_value idx (\<lambda>_. v))) u)}
+                    \<s>\<u>\<b>\<j> u. u \<in> nosep ` {a. index_value idx a = u_idx}
+                      \<and> u \<in> nosep ` Well_Type TY)
+    \<r>\<e>\<f>\<i>\<n>\<e>\<s> {(idx \<^enum>\<^sub>m (map_option nosep \<circ> Map_of_Val u_idx),
+            idx \<^enum>\<^sub>m (map_option nosep \<circ> Map_of_Val v))}
+    \<w>.\<r>.\<t> \<F>_functional Map_of_Val_ins (Map_of_Val_ins_dom TY)
+    \<i>\<n> {idx \<^enum>\<^sub>m (map_option nosep \<circ> Map_of_Val u_idx)}\<close>
+  apply (subst fiction_Map_of_Val_ins_comp_id_simp[symmetric])
+  apply (rule sep_refinement_stepwise[
+            OF refinement_frame[where R = UNIV, OF Map_of_Val_ins.\<F>_functional_refinement_complex[simplified]]])
+  apply (simp add: ExSet_expn Subjection_expn split_nosep_ex inj_image_mem_iff split_option_all
+                   split_nosep_all index_mod_value_welltyp)
+  apply (simp add: frame_preserving_relation_def split_option_all split_nosep_all
+                   ExSet_expn Subjection_expn)
+  apply (simp add: Sep_Closed_def)
+  subgoal premises prems proof -
+    have t1: \<open>B \<subseteq> B' \<Longrightarrow> A * B \<subseteq> A * B'\<close> for A B B'
+      by (clarsimp simp add: subset_iff set_mult_expn; blast)
+    have \<open>pairself Map_of_Val_ins `
+            ({(Some u, (Some \<circ> map_nosep (index_mod_value idx (\<lambda>_. v))) u)} \<s>\<u>\<b>\<j> u.
+             u \<in> nosep ` {a. index_value idx a = u_idx} \<and> u \<in> nosep ` Well_Type TY)
+        \<subseteq> ({(a, a ++ (idx \<^enum>\<^sub>m (map_option nosep \<circ> Map_of_Val v)))} \<s>\<u>\<b>\<j> a. dom a = Dom_of_TY TY)\<close>
+      apply (clarsimp simp add: set_eq_iff ExSet_image Subjection_image;
+             auto simp add: ExSet_expn Subjection_expn split_nosep_ex inj_image_mem_iff)
+      apply (metis Map_of_Val_mod map_option_funcomp_map_add map_option_homo_one prems(1) prems(3) push_map_homo)
+      using Map_of_Val_dom apply blast
+      using Map_of_Val_dom by blast
+    note t2 = this[THEN t1, THEN refinement_sub_fun]
+    have t3: \<open>dom (Map_of_Val v) = Dom_of_TY (index_type idx TY)\<close>
+      using Map_of_Val_dom prems(3) by force
+    have t4: \<open>idx \<^enum>\<^sub>m (map_option nosep \<circ> Map_of_Val u_idx) \<noteq> 1\<close>
+      by (smt (verit) Mapof_not_1 dom_1 dom_eq_empty_conv dom_map_option_comp push_map_eq_1)
+    then have t5: \<open> r * idx \<^enum>\<^sub>m (map_option nosep \<circ> Map_of_Val u_idx) \<noteq> 1\<close> for r
+      by (metis (no_types, opaque_lifting) dom1_disjoint_sep_disj dom1_dom dom_eq_empty_conv empty_subsetI inf.orderE one_partial_map sep_no_inverse times_fun_def times_option_none)
+    show ?thesis
+      apply (rule t2)
+      apply (rule map_tree_refinement_modify)
+      apply (simp add: Dom_of_TY Map_of_Val_dom prems(1) prems(2) prems(4) t3)
+      apply (simp add: Map_of_Val_ins_def Map_of_Val_ins_dom_def image_iff split_option_ex
+                       split_nosep_ex split_nosep_meta_all split_nosep_all t5)
+      by (metis index_mod_value_welltyp prems(1) prems(3) prems(4) val_map_mod_index_value)
+  qed
+  subgoal premises prems proof -
+    have t1: \<open> Domain ({(a u, b u)} \<s>\<u>\<b>\<j> u. P u) = { a u |u. P u }\<close> for a b P
+      unfolding set_eq_iff Domain_unfold by (clarsimp simp add: ExSet_expn Subjection_expn)
+    have t2: \<open>{Some u |u. u \<in> nosep ` {a. index_value idx a = u_idx} \<and> u \<in> nosep ` Well_Type TY}
+                = Some ` nosep ` {a. index_value idx a = u_idx \<and> a \<in> Well_Type TY}\<close>
+      by (clarsimp simp add: set_eq_iff image_iff Bex_def; blast)
+
+    show ?thesis
+      by (subst t1, subst t2, rule val_map_mod_index_value_projection, insert prems(1) prems(4))
+  qed .
+
+
+locale pointer_mem_resource =
+  partial_map_resource Res \<open>\<lambda>blk. nosep ` Well_Type (typ_of_blk blk)\<close>
+  for Res :: "('blk \<Rightarrow> VAL nosep option) resource_entry"
+  and typ_of_blk :: \<open>'blk \<Rightarrow> TY\<close>
+
+locale direct_pointer_mem_fiction =
+  pointwise_base_fiction_for_partial_mapping_resource
+      Res \<open>\<lambda>blk. \<F>_functional Map_of_Val_ins (Map_of_Val_ins_dom (typ_of_blk blk))\<close>
+      Fic \<open>\<lambda>blk. nosep ` Well_Type (typ_of_blk blk)\<close>
+  for Res :: "('blk \<Rightarrow> VAL nosep option) resource_entry"
+  and Fic :: "('blk \<Rightarrow> nat list \<Rightarrow> VAL nosep option) fiction_entry"
+  and typ_of_blk :: \<open>'blk \<Rightarrow> TY\<close>
+begin
+
+sublocale pointer_mem_resource Res typ_of_blk ..
+
+lemmas getter_rule = "_getter_rule_2_"[OF fiction_Map_of_Val_ins_projection',
+                                          simplified split_nosep_ExSet inj_image_mem_iff inj_nosep]
+
+thm fiction_Map_of_Val_ins_refinement
+thm "_setter_rule_2_"[where f=\<open>Some \<circ> map_nosep (index_mod_value idx (\<lambda>_. v))\<close>
+                        and V=\<open>nosep ` {a. index_value idx a = u_idx}\<close>
+                        and F=\<open>\<lambda>_. idx \<^enum>\<^sub>m (map_option nosep \<circ> Map_of_Val v)\<close>
+                        for idx v u_idx,
+                      OF fiction_Map_of_Val_ins_refinement
+                         fiction_Map_of_Val_ins_projection']
+thm fiction_Map_of_Val_ins_projection'
+
+end
+
+
+
+
+
+
+
+
+
+
+
+
+
+
+
+
+
+
+
+
+locale Map_of_Val_insertion = cancl_sep_insertion_monoid \<psi> D
+  for \<psi> :: \<open>'a::{sep_cancel,nonsepable_monoid} \<Rightarrow> 'k list \<Rightarrow> 'b::nonsepable_semigroup option\<close> and D
+begin
+
+lemma refinement_partial_read':
+  \<open> refinement_projection (\<F>_functional \<psi> D) (the_subtree idx ` \<psi> ` {a})
+        \<subseteq> UNIV * {u. the_subtree idx (\<psi> u) = the_subtree idx (\<psi> a) } \<close>
+  unfolding refinement_projection_def
+  apply (clarsimp simp add: set_mult_expn; cases \<open>a = 1\<close>, simp)
+  apply force
+subgoal for x u
+
+lemma refinement_modifcation:
+  \<open> a \<noteq> 1 \<and> pull_map idx (\<psi> a) \<noteq> 1
+\<Longrightarrow> dom (pull_map idx (\<psi> a)) = dom (\<psi> b)
+\<Longrightarrow> a \<in> D \<and> f a b \<in> D
+\<Longrightarrow> \<F>_functional_condition D
+\<Longrightarrow> \<psi> (f a b) = \<psi> a ++ push_map idx (\<psi> b)
+\<Longrightarrow> Id_on UNIV * {(a, f a b)}
+    \<r>\<e>\<f>\<i>\<n>\<e>\<s> {( the_subtree idx (\<psi> a), push_map idx (\<psi> b) )}
+    \<w>.\<r>.\<t> \<F>_functional \<psi> D
+    \<i>\<n> (push_map idx o pull_map idx) ` \<psi> ` {a} \<close>
+  unfolding Fictional_Forward_Simulation_def \<F>_functional_condition_def the_subtree_def
+  apply (clarsimp simp add: set_mult_expn Map_of_Val_mod Subjection_expn sep_disj_partial_map_disjoint)
+  subgoal premises prems for r R u v
+  proof -
+    have \<open>idx \<^enum>\<^sub>m pull_map idx (\<psi> a) \<noteq> 1\<close>
+      by (simp add: prems(5) prems(9))
+    then have \<open>\<psi> v \<noteq> 1\<close>
+      by (metis prems(11) prems(8) prems(9) sep_disj_partial_map_disjoint sep_no_inverse)
+    then have t2: \<open>v \<noteq> 1\<close>
+      by blast
+    have t1: \<open>dom (idx \<^enum>\<^sub>m pull_map idx (\<psi> a)) = dom (idx \<^enum>\<^sub>m \<psi> b)\<close>
+      by (simp add: prems(1) prems(9))
+    have t3: \<open>dom r \<inter> dom (idx \<^enum>\<^sub>m \<psi> b) = {}\<close>
+      using prems(8) prems(9) t1 by force
+     show ?thesis
+       by (insert prems t2, auto simp add: t3, rule exI[where x=1], simp,
+           metis Int_absorb inf.absorb_iff1 map_add_subsumed_dom t1 times_fun_map_add_right)
+   qed .
+
+end
+
+
+interpretation Map_of_Val_ins: Map_of_Val_insertion \<open>Map_of_Val_ins\<close> \<open>Map_of_Val_ins_dom TY\<close>
+  apply (standard; clarsimp simp add: Map_of_Val_ins_def split_nosep_meta_all
+                                      Map_of_Val_ins_dom_def
+                            split: option.split)
+
+  apply (auto simp add: fun_eq_iff split_option_ex times_fun 
+                                  sep_disj_fun_def split_nosep_meta_all
+                        split: option.split)[1]
+  using Mapof_not_1 apply fastforce
+  apply (metis Map_of_Val_same_dom domIff option.map_disc_iff times_option(2))
+  subgoal premises prems for a x x' proof -
+    have t1: \<open>a x = 1\<close> for x
+      by (metis Map_of_Val_same_dom domIff one_option_def option.map_disc_iff prems(1) prems(2) prems(3) prems(4) times_option(2))
+    have t2: \<open>map_option nosep o Map_of_Val x = map_option nosep o Map_of_Val x'\<close>
+      using prems(4) t1 by auto
+    show ?thesis
+      by (metis (mono_tags, lifting) Map_of_Val_inj fun.inj_map_strong nosep.inject option.inj_map_strong prems(2) prems(3) t2) 
+  qed .
+
+lemma \<F>_functional_condition_Map_of_Val_ins_dom:
+  \<open>\<F>_functional_condition (Map_of_Val_ins_dom TY)\<close>
+  unfolding \<F>_functional_condition_def Map_of_Val_ins_dom_def
+  by (clarsimp; case_tac r; case_tac x; simp)
+
+lemma shared_mem_map_refinement_write:
+  \<open> valid_index TY idx
+\<Longrightarrow> u \<in> Well_Type TY \<and> v \<in> Well_Type (index_type idx TY)
+\<Longrightarrow> Id_on UNIV * {(Some (nosep u), Some (nosep (index_mod_value idx (\<lambda>_. v) u)))}
+    \<r>\<e>\<f>\<i>\<n>\<e>\<s> {(to_share \<circ> the_subtree idx (map_option nosep \<circ> Map_of_Val u),
+            to_share \<circ> idx \<^enum>\<^sub>m (map_option nosep \<circ> Map_of_Val v))}
+    \<w>.\<r>.\<t> \<F>_functional ((\<circ>) to_share o Map_of_Val_ins) (Map_of_Val_ins_dom TY)
+    \<i>\<n> {to_share \<circ> the_subtree idx (map_option nosep \<circ> Map_of_Val u)}\<close>
+unfolding the_subtree_def
+subgoal premises prems
+proof -
+  have s: \<open>\<F>_functional ((\<circ>) to_share o Map_of_Val_ins) (Map_of_Val_ins_dom TY)
+          = \<F>_functional Map_of_Val_ins (Map_of_Val_ins_dom TY) \<Zcomp>\<^sub>\<I> \<F>_functional ((\<circ>) to_share) UNIV\<close>
+    by (rule \<F>_functional_comp, simp add: subset_iff)
+
+  have t1[simp]: \<open>f ` {x} = { f x }\<close> for f x by simp
+  note pointwise_set_UNIV[simp]
+       \<F>_functional_condition_Map_of_Val_ins_dom[simp]
+  note rule = sep_refinement_stepwise[
+        OF refinement_frame[OF
+            Map_of_Val_ins.refinement_modifcation
+              [where a=\<open>Some (nosep u)\<close> and b=\<open>Some (nosep v)\<close> and idx = idx
+                and f = \<open>\<lambda>u' v'. Some (nosep (index_mod_value idx (\<lambda>_. nosep.dest (the v')) (nosep.dest (the u'))))\<close>,
+               simplified, simplified t1 the_subtree_def, simplified]]
+            pointwise_to_share.\<F>_functional_refinement[simplified]
+            pointwise_to_share.\<F>_functional_projection
+              [where S=\<open>{idx \<^enum>\<^sub>m pull_map idx (map_option nosep \<circ> Map_of_Val u)}\<close>, simplified]]
+  have t2[simp]: \<open>pull_map idx (map_option nosep \<circ> Map_of_Val u) = map_option nosep \<circ> (Map_of_Val (index_value idx u))\<close>
+    by (simp add: pull_map_funcomp[symmetric] Map_of_Val_pull[OF prems(1) prems(2)[THEN conjunct1]])
+
+  thm pointwise_to_share.refinement_projection_half_perm[simplified]
+  thm refinement_projections_stepwise
+  thm Map_of_Val_ins.\<F>_functional_projection[simplified]
+  thm Map_of_Val_ins.\<F>_functional_projection[simplified]
+
+  show ?thesis
+    apply (subst s, rule rule)
+    using t2 Mapof_not_1 comp_eq_dest_lhs apply fastforce
+    apply (unfold t2 dom_map_option_comp, meson Map_of_Val_same_dom index_value_welltyp prems(1) prems(2) t2)
+    apply (simp add: index_mod_value_welltyp prems(1) prems(2))
+    by (metis Map_of_Val_mod map_option_funcomp_map_add map_option_homo_one prems(1) prems(2) push_map_homo) 
+qed .
+
+
+(*
+lemma refinement_partial_read:
+  \<open> valid_index TY idx
+\<Longrightarrow> u \<in> Well_Type TY
+\<Longrightarrow> refinement_projection (\<F>_functional Map_of_Val_ins (Map_of_Val_ins_dom TY))
+          (the_subtree idx ` Map_of_Val_ins ` {Some (nosep u)}) \<subseteq> UNIV * {Some (nosep u)} \<close>
+thm Map_of_Val_ins.refinement_partial_read'
+  apply (rule Map_of_Val_ins.refinement_partial_read')
+  apply (clarsimp simp add: set_mult_expn Map_of_Val_ins_def Map_of_Val_ins_dom_def;
+          case_tac x; simp add: split_nosep_meta_all)
+apply (simp add: the_subtree_def pull_map_funcomp[symmetric])
+  apply (smt (verit, best) Map_of_Val_pull Mapof_not_1 dom_1 dom_eq_empty_conv dom_map_option_comp)
+term Complete_Lattices.Sup_class.Sup  *)
+
+
+lemma map_tree_modify:
+  \<open> D' \<subseteq> D
+\<Longrightarrow> Id_on UNIV * {(a, a ++ push_map idx b) | a b. dom a = D \<and> dom b = D'}
+    \<r>\<e>\<f>\<i>\<n>\<e>\<s> {(a,b). dom a = D' \<and> dom b = D' }
+    \<w>.\<r>.\<t> \<F>_it
+    \<i>\<n> e\<close>
+  for a :: \<open>'a list \<Rightarrow> VAL nosep option\<close>
+
+
+
+
+lemma
+  \<open> refinement_projection (\<F>_functional id {x. dom1 x = dom1 u}) {v} \<subseteq> {u}\<close>
+  for v :: \<open>'a \<Rightarrow> 'b::nonsepable_monoid\<close>
+  unfolding refinement_projection_def
+  apply (clarsimp simp add: set_mult_expn)
+subgoal for w apply (exI[where x=])
+  subgoal for t u' v'
+apply (rule exI[where x=])
+
+
+lemma
+  \<open> valid_index TY idx
+\<Longrightarrow> u \<in> Well_Type TY \<and> v \<in> Well_Type (index_type idx TY)
+\<Longrightarrow> Id_on UNIV * {(Some (nosep u), Some (nosep (index_mod_value idx (\<lambda>_. v) u)))}
+    \<r>\<e>\<f>\<i>\<n>\<e>\<s> pairself (push_map idx o pull_map idx o (o) (map_option nosep) o Map_of_Val) `
+          {(u, index_mod_value idx (\<lambda>_. v) u)}
+    \<w>.\<r>.\<t> \<F>_functional Map_of_Val_ins (Map_of_Val_ins_dom TY) \<Zcomp>\<^sub>\<I> \<F>_functional id {x. dom x \<subseteq> dom (Map_of_Val u)}
+    \<i>\<n> (push_map idx o pull_map idx o (o) (map_option nosep) o Map_of_Val) ` {u}\<close>
+  apply (rule sep_refinement_stepwise)
+  apply (rule refinement_frame[where R=UNIV, OF Map_of_Val_ins.\<F>_functional_refinement[simplified]],
+         simp add: index_mod_value_welltyp,
+         simp add: Map_of_Val_mod map_option_funcomp_map_add push_map_homo)
+  subgoal premises prems proof -
+    have t1: \<open>pull_map idx ((map_option nosep \<circ> Map_of_Val u) ++ (idx \<^enum>\<^sub>m (map_option nosep \<circ> Map_of_Val v)))
+          = map_option nosep \<circ> Map_of_Val v \<close>
+      apply (clarsimp simp add: pull_map_map_add)
+      by (metis (no_types, lifting) Map_of_Val_pull Map_of_Val_same_dom dom_map_option_comp index_value_welltyp map_add_subsumed_dom prems(1) prems(2) pull_map_dom_eq subsetI)
+    show ?thesis
+      apply (simp add: t1)
+      apply (rule map_tree_modify[where a=\<open>map_option nosep \<circ> Map_of_Val u\<close> and b=\<open>map_option nosep \<circ> Map_of_Val v\<close>, simplified])
+      by (metis Map_of_Val_pull Map_of_Val_same_dom dom_map_option_comp index_value_welltyp prems(1) prems(2) pull_map_dom_eq)
+  qed
+  apply simp
+proof -
+have \<open>dom (idx \<^enum>\<^sub>m pull_map idx (map_option nosep \<circ> Map_of_Val u)) \<subseteq> dom (map_option nosep \<circ> Map_of_Val u)\<close>
+  by (meson map_le_implies_dom_le push_pull_map)
+  apply (clarsimp simp add: refinement_projection_def set_mult_expn)
+apply simp
+thm map_tree_modify[where a=\<open>map_option nosep \<circ> Map_of_Val u\<close> and b=\<open>map_option nosep \<circ> Map_of_Val v\<close>]
+thm map_tree_modify
+
+thm map_option_funcomp_map_add pull_map_map_add push_map_distrib_map_add
+
+apply (rule map_tree_modify)
+
+thm Map_of_Val_ins.push_map_homo
+
+
+  thm Map_of_Val_mod
+
+term \<open>a o (b ++ c)\<close>
+
+thm Map_of_Val_ins.\<F>_functional_refinement[simplified,
+      where a=\<open>Some (nosep u)\<close> and b=\<open>Some (nosep v)\<close>]
+thm Map_of_Val_ins.\<F>_functional_refinement[simplified,
+      where a=\<open>Some (nosep u)\<close> and b=\<open>Some (nosep v)\<close>,
+      simplified,
+      where v1=\<open>index_mod_value idx (\<lambda>_. w) v\<close> for idx w v,
+      simplified Map_of_Val_mod]
+thm sep_refinement_stepwise[
+      OF Map_of_Val_ins.\<F>_functional_refinement[simplified,
+            where a=\<open>Some (nosep u)\<close> and b=\<open>Some (nosep v)\<close> for u v,
+            simplified,
+            where v1=\<open>index_mod_value idx (\<lambda>_. u) v\<close> for idx u v]
+                               ]
+thm map_tree_modify
+thm Map_of_Val_mod
+
+
+
+
 
 term \<open>((o) (map_option nosep)) o Map_of_Val' o map_option nosep.dest\<close>
 term \<open>map_option nosep.dest\<close>
